
$$
\begin{align}
\overline{|u(t)|} &= \frac{1}{T} \left(\int^\frac{T}{2}_{0}|U_{A}|\,dt + \int ^T_{\frac{T}{2}} |-U_{A}|\, dt\right) \\
&= \frac{1}{T} \int _{0}^T U_{A} \, dt \\
&= \frac{1}{T}\cdot (U_{A}\cdot T-U_{A} \cdot 0) = U_{A} 
\end{align}
$$

$$
\begin{align}
\overline{|u(t)|} &= \frac{1}{T}\left( \int _{0}^\frac{T}{2} |U_{A}| \, dt +\int _{\frac{T}{2}}^T 0\, dx \right) \\
&= \frac{1}{T} \left(U_{A}\cdot \frac{T}{2}-U_{A} \cdot 0+ 0\cdot 0-0 \cdot\frac{T}{2}\right) \\
&= \frac{U_{A}}{2} 
\end{align}
$$

